If we look at the case of logistic regression, we know that $h_w(x) = \Theta(w^T x)$, where
\begin{align}
\Theta(s) = \frac{e^s}{1+e^s}
\end{align}
By simpel calculation we get that
\begin{align}
1 - \Theta(s) = 1 - \frac{e^s}{1+e^s} = \frac{e^{-s}}{1+e^{-s}} = \Theta(-s)
\end{align}
which means that

...

We therefore have that
\begin{align}

\end{align}

for $y\in \{-1,1 \}$ and all $x\in \mathcal{X}$.

\begin{align}
[[y_n = 1]]\left(\ln \left( \frac{1}{h_w(x_n)}\right)\right) + [[y_n = -1]]\left(\ln \left( \frac{1}{1 - h_w(x_n)}\right)\right) = \\ 
[[y_n = 1]]\left(\ln \left( \frac{1}{h_w(x_n)}\right)\right) + [[y_n = -1]]\left(\ln \left( \frac{1}{1 - h_w(x_n)}\right)\right)
\end{align}